Update SHA512 proofs after planning session with Alex/Sid

Proofs/SHA512/SHA512Loop.lean
@@ -14,35 +14,49 @@ is satisfied.
 
 namespace SHA512
 
-structure sha512_loop_post (nblocks : BitVec 64) (si : ArmState) : Prop where
+-- (TODO @shilpi) Write the loop invariant.
+
+structure sha512_loop_post
+  (pc nblocks sp ctx_base input_base : BitVec 64)
+  (si : ArmState) : Prop where
   h_program    : si.program = program
+  h_pc         : r .PC si = pc
   h_err        : r .ERR si = .None
-  -- (FIXME) PC should be 0x126c94#64 i.e., we are poised to execute the first
-  -- instruction following the loop.
-  h_pc         : r .PC si = 0x1268e8#64
   h_sp_aligned : CheckSPAlignment si
+  -- No blocks must be left unhashed by the time the loop runs to completion.
   h_num_blocks : num_blocks si = 0#64
-  -- h_ktbl_addr  : r (.GPR 3#5) si = ktbl_addr
-  -- h_ctx        : si[ctx_addr si, 64] = SHA2.h0_512.toBitVec
-  -- h_ktbl       : si[ktbl_addr, (SHA2.k_512.length * 8)] = BitVec.flatten SHA2.k_512
-  -- h_mem_sep    : Memory.Region.pairwiseSeparate
-  --                 [(stack_ptr si,   16),
-  --                  (ctx_addr si,    64),
-  --                  (input_addr si - 128#64, ((num_blocks si).toNat * 128)),
-  --                  (ktbl_addr,      (SHA2.k_512.length * 8))]
+  h_sp         : stack_ptr si = sp - 16#64
+  h_ctx_base   : ctx_addr si = ctx_base
+  h_input_base : input_addr si = input_base
+  -- (TODO @shilpi) The ctx must contain the hash.
+  -- h_ctx        : si[ctx_base, 64] = SHA2.h0_512.toBitVec
+  h_ktbl       : si[ktbl_addr, (SHA2.k_512.length * 8)] = BitVec.flatten SHA2.k_512
+  h_mem_sep    : Memory.Region.pairwiseSeparate
+                  [(sp - 16#64,   16),
+                   (ctx_base,     64),
+                   (input_base,   (nblocks.toNat * 128)),
+                   (ktbl_addr,    (SHA2.k_512.length * 8))]
 
 theorem sha512_loop_post.iff_def :
-  (sha512_loop_post nblocks si) ↔
+  (sha512_loop_post pc nblocks sp ctx_base input_base si) ↔
   (si.program = program ∧
+   r .PC si = pc ∧
    r .ERR si = .None ∧
-  -- (FIXME) PC should be 0x126c94#64 i.e., we are poised to execute the first
-  -- instruction following the loop.
-   r .PC si = 0x1268e8#64 ∧
    CheckSPAlignment si ∧
-   num_blocks si = 0#64) := by
+   num_blocks si = 0#64 ∧
+   stack_ptr si = sp - 16#64 ∧
+   ctx_addr si = ctx_base ∧
+   input_addr si = input_base ∧
+  --  si[ctx_base, 64] = SHA2.h0_512.toBitVec ∧
+   si[ktbl_addr, (SHA2.k_512.length * 8)] = BitVec.flatten SHA2.k_512 ∧
+   Memory.Region.pairwiseSeparate
+                 [(sp - 16#64,   16),
+                  (ctx_base,     64),
+                  (input_base,   (nblocks.toNat * 128)),
+                  (ktbl_addr,    (SHA2.k_512.length * 8))]) := by
   constructor
   · intro h
-    obtain ⟨h_program, h_err, h_pc, h_sp_aligned, h_num_blocks⟩ := h
+    obtain ⟨⟩ := h
     simp only [*, minimal_theory]
   · intro h
     constructor <;> simp only [*, minimal_theory]
@@ -55,27 +69,42 @@ branch here:
 -- (0x126c90#64 , 0xb5ffc382#32) --  cbnz    x2, 126500 <sha512_block_armv8+0x40>
 -/
 set_option linter.unusedVariables false in
+set_option debug.skipKernelTC true in
 -- set_option trace.Tactic.sym.heartbeats true in
 -- set_option profiler true in
 -- set_option profiler.threshold 1 in
-theorem sha512_block_armv8_loop_1block (s0 sf : ArmState)
-  (h_s0_prelude : sha512_prelude 1#64 s0)
-  (h_run : sf = run 250 s0) :
-  sha512_loop_post 0#64 sf := by
+set_option maxHeartbeats 0 in
+-- set_option maxRecDepth 0 in
+theorem sha512_block_armv8_loop_1block (si sf : ArmState)
+  (h_N : N = 1#64)
+  (h_si_prelude : sha512_prelude 0x126500#64 N SP CtxBase InputBase si)
+  -- TODO: Ideally, nsteps ought to be 485 to be able to simulate the loop to
+  -- completion.
+  (h_steps : nsteps = 20)
+  (h_run : sf = run nsteps si) :
+  -- (FIXME) PC should be 0x126c94#64 i.e., we are poised to execute the first
+  -- instruction following the loop. For now, we stop early on to remain in sync.
+  -- with the number of steps we simulate.
+  sha512_loop_post (0x126500#64 + nsteps*4)
+     N SP CtxBase InputBase sf := by
   -- Prelude
-  obtain ⟨h_s0_program, h_s0_err, h_s0_pc, h_s0_sp_aligned,
-          h_s0_num_blocks, h_s0_x3, h_s0_ctx,
-          h_s0_ktbl, h_s0_separate⟩ := h_s0_prelude
+  subst h_N h_steps
+  obtain ⟨h_si_program, h_si_pc, h_si_err, h_si_sp_aligned,
+          h_si_num_blocks, h_si_sp, h_si_ctx_base,
+          h_si_input_base, h_si_ctx, h_si_ktbl, h_si_separate⟩ := h_si_prelude
   simp only [num_blocks, ctx_addr, stack_ptr, input_addr] at *
   simp only [sha512_loop_post.iff_def]
   -- Symbolic Simulation
-  sym_n 250
+  sym_n 20
   -- Epilogue
   -- cse (config := { processHyps := .allHyps })
-  simp (config := {decide := true})  only
-        [fst_AddWithCarry_eq_add, fst_AddWithCarry_eq_sub_neg,
-         h_s0_num_blocks,
+  simp (config := {ground := true}) only
+        [fst_AddWithCarry_eq_sub_neg,
+         ConditionHolds,
+         state_simp_rules,
          bitvec_rules, minimal_theory]
+  sym_aggregate
+  exact ⟨h_si_ktbl, h_si_separate⟩
   done
 
 end SHA512
