Proofs/SHA512/SHA512Prelude.lean
@@ -36,84 +36,114 @@ abbrev num_blocks (s : ArmState) : BitVec 64 := r (StateField.GPR 2#5) s
 -- (0x1264d8#64 , 0x910c0063#32),      --  add     x3, x3, #0x300
 abbrev ktbl_addr : BitVec 64 := 0x1b4300#64
 
+/--
+Preconditions for the simulation of SHA512.
+-/
+structure sha512_init_pre
+    (pc nblocks sp ctx_base input_base : BitVec 64)
+    (s0 : ArmState) : Prop where
+  h_program    : s0.program = program
+  h_pc         : read_pc s0 = pc
+  h_err        : read_err s0 = .None
+  h_sp_aligned : CheckSPAlignment s0
+  h_num_blocks : num_blocks s0 = nblocks
+  h_sp         : stack_ptr s0 = sp
+  h_ctx_base   : ctx_addr s0 = ctx_base
+  h_input_base : input_addr s0 = input_base
+  h_ctx        : s0[ctx_addr s0, 64] = SHA2.h0_512.toBitVec
+  h_ktbl       : s0[ktbl_addr, (SHA2.k_512.length * 8)] = BitVec.flatten SHA2.k_512
+  h_mem_sep    : Memory.Region.pairwiseSeparate
+                  [((sp - 16#64), 16),
+                   (ctx_base,     64),
+                   (input_base,   (nblocks.toNat * 128)),
+                   (ktbl_addr,    (SHA2.k_512.length * 8))]
 
-private theorem add_eq_sub_16 (x : BitVec 64) :
-  x + 0xfffffffffffffff0#64 = x - 16#64 := by
-  bv_decide
-
-structure sha512_prelude (nblocks : BitVec 64) (si : ArmState) : Prop where
+/--
+Invariant that must hold after SHA512's first basic block is simulated, i.e.,
+the basic block immediately preceding the loop.
+-/
+structure sha512_prelude
+    (pc nblocks sp ctx_base input_base : BitVec 64)
+    (si : ArmState) : Prop where
   h_program    : si.program = program
+  h_pc         : r .PC si = pc
   h_err        : r .ERR si = .None
-  h_pc         : r .PC si = 0x126500#64
   h_sp_aligned : CheckSPAlignment si
   h_num_blocks : num_blocks si = nblocks
-  h_ktbl_addr  : r (.GPR 3#5) si = ktbl_addr
-  -- ctx_addr si = ctx_addr s
-  -- input_addr si = input_addr s + 128#64
-  -- stack_ptr si = stack_ptr s - 16#64
-  h_ctx        : si[ctx_addr si, 64] = SHA2.h0_512.toBitVec
+  h_sp         : stack_ptr si = sp - 16#64
+  h_ctx_base   : ctx_addr si = ctx_base
+  h_input_base : input_addr si = input_base + 128#64
+  h_ctx        : si[ctx_base, 64] = SHA2.h0_512.toBitVec
   h_ktbl       : si[ktbl_addr, (SHA2.k_512.length * 8)] = BitVec.flatten SHA2.k_512
   h_mem_sep    : Memory.Region.pairwiseSeparate
-                  [(stack_ptr si,   16),
-                   (ctx_addr si,    64),
-                   (input_addr si - 128#64, ((num_blocks si).toNat * 128)),
-                   (ktbl_addr,      (SHA2.k_512.length * 8))]
+                  [(sp - 16#64,   16),
+                   (ctx_base,     64),
+                   (input_base,   (nblocks.toNat * 128)),
+                   (ktbl_addr,    (SHA2.k_512.length * 8))]
 
-theorem sha512_prelude.def (h : sha512_prelude nblocks si) :
+theorem sha512_prelude.def
+  (h : sha512_prelude pc nblocks sp ctx_base input_base si) :
   si.program = program ∧
+  r .PC si = pc ∧
   r .ERR si = .None ∧
-  r .PC si = 0x126500#64 ∧
   CheckSPAlignment si ∧
   num_blocks si = nblocks ∧
-  r (.GPR 3#5) si = ktbl_addr ∧
-  si[ctx_addr si, 64] = SHA2.h0_512.toBitVec ∧
+  stack_ptr si = sp - 16#64 ∧
+  ctx_addr si = ctx_base ∧
+  input_addr si = input_base + 128#64 ∧
+  si[ctx_base, 64] = SHA2.h0_512.toBitVec ∧
   si[ktbl_addr, (SHA2.k_512.length * 8)] = BitVec.flatten SHA2.k_512 ∧
   Memory.Region.pairwiseSeparate
-            [(stack_ptr si,   16),
-             (ctx_addr si,    64),
-             (input_addr si - 128#64, ((num_blocks si).toNat * 128)),
-             (ktbl_addr,      (SHA2.k_512.length * 8))] := by
-  obtain ⟨h1, h2, h3, h4, h5, h6, h7, h8, h9⟩ := h
+            [(sp - 16#64, 16),
+             (ctx_base,   64),
+             (input_base, (nblocks.toNat * 128)),
+             (ktbl_addr,  (SHA2.k_512.length * 8))] := by
+  obtain ⟨⟩ := h
   repeat' apply And.intro
   repeat assumption
   done
 
 theorem sha512_prelude.of_def
   (h : si.program = program ∧
+       r .PC si = pc ∧
        r .ERR si = .None ∧
-       r .PC si = 0x126500#64 ∧
        CheckSPAlignment si ∧
        num_blocks si = nblocks ∧
-       r (.GPR 3#5) si = ktbl_addr ∧
-       si[ctx_addr si, 64] = SHA2.h0_512.toBitVec ∧
+       stack_ptr si = sp - 16#64 ∧
+       ctx_addr si = ctx_base ∧
+       input_addr si = input_base + 128#64 ∧
+       si[ctx_base, 64] = SHA2.h0_512.toBitVec ∧
        si[ktbl_addr, (SHA2.k_512.length * 8)] = BitVec.flatten SHA2.k_512 ∧
        Memory.Region.pairwiseSeparate
-                [(stack_ptr si,   16),
-                 (ctx_addr si,    64),
-                 (input_addr si - 128#64, ((num_blocks si).toNat * 128)),
-                 (ktbl_addr,      (SHA2.k_512.length * 8))]) :
-  sha512_prelude nblocks si := by
-  obtain ⟨h_program, h_err, h_pc, h_sp_aligned, h_num_blocks, h_ktbl_addr,
-          h_ctx, h_ktbl, h_mem_sep⟩ := h
+                 [(sp - 16#64, 16),
+                  (ctx_base,   64),
+                  (input_base, (nblocks.toNat * 128)),
+                  (ktbl_addr,  (SHA2.k_512.length * 8))]) :
+         sha512_prelude pc nblocks sp ctx_base input_base si := by
+  obtain ⟨h_program, h_pc, h_err, h_sp_aligned, h_num_blocks,
+          h_sp, h_ctx_base, h_input_base, h_ctx, h_ktbl,
+          h_mem_sep⟩ := h
   constructor
   repeat assumption
   done
 
 theorem sha512_prelude.iff_def :
-  (sha512_prelude nblocks si) ↔
+  (sha512_prelude pc nblocks sp ctx_base input_base si) ↔
   (si.program = program ∧
+   r .PC si = pc ∧
    r .ERR si = .None ∧
-   r .PC si = 0x126500#64 ∧
    CheckSPAlignment si ∧
    num_blocks si = nblocks ∧
-   r (.GPR 3#5) si = ktbl_addr ∧
-   si[ctx_addr si, 64] = SHA2.h0_512.toBitVec ∧
+   stack_ptr si = sp - 16#64 ∧
+   ctx_addr si = ctx_base ∧
+   input_addr si = input_base + 128#64 ∧
+   si[ctx_base, 64] = SHA2.h0_512.toBitVec ∧
    si[ktbl_addr, (SHA2.k_512.length * 8)] = BitVec.flatten SHA2.k_512 ∧
    Memory.Region.pairwiseSeparate
-            [(stack_ptr si,   16),
-             (ctx_addr si,    64),
-             (input_addr si - 128#64, ((num_blocks si).toNat * 128)),
-             (ktbl_addr,      (SHA2.k_512.length * 8))]) := by
+             [(sp - 16#64, 16),
+              (ctx_base,   64),
+              (input_base, (nblocks.toNat * 128)),
+              (ktbl_addr,  (SHA2.k_512.length * 8))]) := by
   constructor
   · apply sha512_prelude.def
   · intro h
@@ -121,27 +151,27 @@ theorem sha512_prelude.iff_def :
     assumption
   done
 
+private theorem add_eq_sub_16 (x : BitVec 64) :
+  x + 0xfffffffffffffff0#64 = x - 16#64 := by
+  bv_decide
+
+-- Convention: Use PascalCase for "constants". E.g., `N`, `SP`, `CtxBase`, and
+-- `InputBase` below always refer to projections of the initial state `s0`.
+
+-- (TODO) Modifying this theorem is an exercise in patience because of
+-- user-interactivity delays. Let's report this.
 theorem sha512_block_armv8_prelude (s0 sf : ArmState)
-  (h_s0_pc : read_pc s0 = 0x1264c0#64)
-  (h_s0_err : read_err s0 = StateError.None)
-  (h_s0_sp_aligned : CheckSPAlignment s0)
-  (h_s0_program : s0.program = program)
   -- We fix the number of blocks to hash to 1.
-  (h_s0_num_blocks : num_blocks s0 = 1#64)
-  (_h_s0_x3 : r (StateField.GPR 3#5) s0 = ktbl_addr)
-  (h_s0_ctx : read_mem_bytes 64 (ctx_addr s0) s0 = SHA2.h0_512.toBitVec)
-  (h_s0_ktbl : read_mem_bytes (SHA2.k_512.length * 8) ktbl_addr s0 = BitVec.flatten SHA2.k_512)
-  (h_s0_separate :
-    Memory.Region.pairwiseSeparate
-    [((stack_ptr s0 - 16#64),   16),
-     (ctx_addr s0,    64),
-     (input_addr s0,  ((num_blocks s0).toNat * 128)),
-     (ktbl_addr,      (SHA2.k_512.length * 8))])
+  (h_N : N = 1#64)
+  (h_s0_init : sha512_init_pre 0x1264c0#64
+                               N SP CtxBase InputBase s0)
   (h_run : sf = run 16 s0) :
-  sha512_prelude (num_blocks s0) sf ∧
-  ctx_addr sf = ctx_addr s0 ∧
-  input_addr sf = input_addr s0 + 128#64 ∧
-  stack_ptr sf = stack_ptr s0 - 16#64 := by
+  sha512_prelude 0x126500#64 N SP CtxBase InputBase sf := by
+  -- Prelude
+  obtain ⟨h_s0_program, h_s0_pc, h_s0_err, h_s0_sp_aligned,
+          h_s0_num_blocks, h_s0_sp, h_s0_ctx_base,
+          h_s0_input_base, h_s0_ctx, h_s0_ktbl,
+          h_s0_mem_sep⟩ := h_s0_init
   -- Symbolic Simulation
   sym_n 1
   case h_s1_sp_aligned =>
@@ -161,23 +191,23 @@ theorem sha512_block_armv8_prelude (s0 sf : ArmState)
     apply Aligned_BitVecAdd_64_4 h_s0_sp_aligned (by decide)
   sym_n 15 at s1
   -- Epilogue
-  simp only [num_blocks, stack_ptr, ctx_addr, input_addr, ←add_eq_sub_16] at *
+  -- simp only [num_blocks, stack_ptr, ctx_addr, input_addr, ←add_eq_sub_16] at *
+  simp only [←add_eq_sub_16] at *
   -- cse (config := { processHyps := .allHyps })
-  simp (config := {decide := true}) only
-        [h_s0_num_blocks, h_s0_ktbl,
-         AddWithCarry, stack_ptr, input_addr,
-         bitvec_rules, minimal_theory]
-  -- The following discharges
-  --  r (StateField.GPR 0x1#5) s0 + 0x40#64 + 0x40#64 =
-  --  r (StateField.GPR 0x1#5) s0 + 0x80#64
-  simp only [BitVec.add_assoc, bitvec_rules, minimal_theory]
+  simp only [sha512_prelude.iff_def, bitvec_rules, minimal_theory]
   -- Opening up `sha512_prelude`:
-  simp only [sha512_prelude.iff_def, num_blocks, ctx_addr]
   -- (FIXME @alex) Why does `s16.program = program` remain even after aggregation?
   sym_aggregate
-  simp only [h_s16_program, minimal_theory]
+  simp only [h_s16_program, ←add_eq_sub_16, minimal_theory]
+  -- The following discharges
+  --  InputBase + 0x40#64 + 0x40#64 =
+  --  InputBase + 0x80#64
+  -- (TODO @bollu) canonicalization: move constants to the left.
+  -- Also upstream, please.
+  simp only [BitVec.add_assoc, bitvec_rules, minimal_theory]
   -- Only memory-related obligations are left.
-  -- Eliminating ∀ in memory non-effect hyps.
+  -- (TODO @alex/@bollu) Remove ∀ in memory (non)effect hyps generated by
+  -- `sym_n`. The user may still state memory properties using quantifiers.
   simp only [←Memory.mem_eq_iff_read_mem_bytes_eq] at *
   -- Rewrite *_mem_bytes (in terms of ArmState) to *_bytes (in terms of Memory).
   simp only [memory_rules] at *
@@ -198,24 +228,30 @@ theorem sha512_block_armv8_prelude (s0 sf : ArmState)
              h_s3_memory_effects,
              h_s2_memory_effects,
              h_s1_memory_effects]
+  -- (NOTE @bollu) The following need to be opened up for `simp_mem`,
+  -- apparently. Is this a big deal though? Maybe not?
+  -- Sid says this is probably because omega is unable to see through the
+  -- defs.
+  simp only [num_blocks, stack_ptr, ctx_addr, input_addr] at *
   constructor
-  · simp_mem
-    simp only [Nat.sub_self, bitvec_rules]
-    -- (FIXME @bollu) `extractLsBytes_eq_self` is in `bitvec_rules` but still,
-    -- we had to apply it below.
-    apply extractLsBytes_eq_self
-  · simp only [h_s0_num_blocks, bitvec_rules] at h_s0_separate
-    constructor
+  · -- (TODO @bollu) Think about whether `simp_mem` should be powerful enough to solve this goal.
+    -- Also, `mem_omega` name suggestion from Alex for the already souped up `simp_mem`.
+    simp_mem
+    simp only [h_s0_ctx_base, Nat.sub_self, bitvec_rules]
+  · constructor
     · -- (FIXME @bollu) simp_mem doesn't make progress here. :-(
+      -- simp only [←h_s0_sp] at h_s0_mem_sep
       rw [Memory.read_bytes_write_bytes_eq_read_bytes_of_mem_separate']
       simp only [h_s0_ktbl]
       -- (FIXME @bollu) Memory.Region.separate'_of_pairwiseSeprate_of_mem_of_mem
-      -- works here, but using it is painful.
-      have := Memory.Region.separate'_of_pairwiseSeprate_of_mem_of_mem h_s0_separate 3 0 (by decide)
+      -- works here, but using it is painful. Also, mispelled lemma.
+      have := Memory.Region.separate'_of_pairwiseSeprate_of_mem_of_mem
+              h_s0_mem_sep 3 0 (by decide)
               (ktbl_addr, (SHA2.k_512.length * 8))
-              ((r (StateField.GPR 0x1f#5) s0 + 0xfffffffffffffff0#64), 16)
+              ((SP + 0xfffffffffffffff0#64), 16)
       simp at this
-      simp only [this]
-    · simp only [h_s0_separate,
+      simp only [h_s0_sp, this]
+    · simp only [h_s0_sp, h_s0_num_blocks, h_s0_input_base, h_s0_ctx_base,
+                 h_s0_mem_sep,
                  BitVec.add_assoc, BitVec.add_sub_cancel, bitvec_rules, minimal_theory]
   done
